Veir/Rewriter/GetSet/InsertOp.lean
@@ -54,80 +54,80 @@ namespace Veir
 
 variable {OpInfo} [HasOpInfo OpInfo]
 variable {ctx : IRContext OpInfo}
-section Rewriter.insertOp?
+section Rewriter.insertOp
 
-unseal Rewriter.insertOp?
+unseal Rewriter.insertOp
 
-attribute [local grind] Rewriter.insertOp?
+attribute [local grind] Rewriter.insertOp
 
 @[simp]
-theorem BlockPtr.firstUse!_insertOp? {block : BlockPtr} :
-    Rewriter.insertOp? ctx newOp ip h₁ h₂ h₃ = some newCtx →
+theorem BlockPtr.firstUse!_insertOp {block : BlockPtr} :
+    Rewriter.insertOp ctx newOp ip h₁ h₂ h₃ = some newCtx →
     (block.get! newCtx).firstUse = (block.get! ctx).firstUse := by
-  simp only [Rewriter.insertOp?]
+  simp only [Rewriter.insertOp]
   grind
 
-grind_pattern BlockPtr.firstUse!_insertOp? =>
-  Rewriter.insertOp? ctx newOp ip h₁ h₂ h₃, some newCtx, (block.get! newCtx).firstUse
+grind_pattern BlockPtr.firstUse!_insertOp =>
+  Rewriter.insertOp ctx newOp ip h₁ h₂ h₃, some newCtx, (block.get! newCtx).firstUse
 
 @[simp]
-theorem BlockPtr.prev!_insertOp? {block : BlockPtr} :
-    Rewriter.insertOp? ctx newOp ip h₁ h₂ h₃ = some newCtx →
+theorem BlockPtr.prev!_insertOp {block : BlockPtr} :
+    Rewriter.insertOp ctx newOp ip h₁ h₂ h₃ = some newCtx →
     (block.get! newCtx).prev = (block.get! ctx).prev := by
-  simp only [Rewriter.insertOp?]
+  simp only [Rewriter.insertOp]
   grind
 
-grind_pattern BlockPtr.prev!_insertOp? =>
-  Rewriter.insertOp? ctx newOp ip h₁ h₂ h₃, some newCtx, (block.get! newCtx).prev
+grind_pattern BlockPtr.prev!_insertOp =>
+  Rewriter.insertOp ctx newOp ip h₁ h₂ h₃, some newCtx, (block.get! newCtx).prev
 
 @[simp]
-theorem BlockPtr.next!_insertOp? {block : BlockPtr} :
-    Rewriter.insertOp? ctx newOp ip h₁ h₂ h₃ = some newCtx →
+theorem BlockPtr.next!_insertOp {block : BlockPtr} :
+    Rewriter.insertOp ctx newOp ip h₁ h₂ h₃ = some newCtx →
     (block.get! newCtx).next = (block.get! ctx).next := by
-  simp only [Rewriter.insertOp?]
+  simp only [Rewriter.insertOp]
   grind
 
-grind_pattern BlockPtr.next!_insertOp? =>
-  Rewriter.insertOp? ctx newOp ip h₁ h₂ h₃, some newCtx, (block.get! newCtx).next
+grind_pattern BlockPtr.next!_insertOp =>
+  Rewriter.insertOp ctx newOp ip h₁ h₂ h₃, some newCtx, (block.get! newCtx).next
 
 @[simp]
-theorem BlockPtr.parent!_insertOp? {block : BlockPtr} :
-    Rewriter.insertOp? ctx newOp ip h₁ h₂ h₃ = some newCtx →
+theorem BlockPtr.parent!_insertOp {block : BlockPtr} :
+    Rewriter.insertOp ctx newOp ip h₁ h₂ h₃ = some newCtx →
     (block.get! newCtx).parent = (block.get! ctx).parent := by
-  simp only [Rewriter.insertOp?]
+  simp only [Rewriter.insertOp]
   grind
 
-grind_pattern BlockPtr.parent!_insertOp? =>
-  Rewriter.insertOp? ctx newOp ip h₁ h₂ h₃, some newCtx, (block.get! newCtx).parent
+grind_pattern BlockPtr.parent!_insertOp =>
+  Rewriter.insertOp ctx newOp ip h₁ h₂ h₃, some newCtx, (block.get! newCtx).parent
 
-theorem BlockPtr.firstOp!_insertOp? {block : BlockPtr} :
-    Rewriter.insertOp? ctx newOp ip h₁ h₂ h₃ = some newCtx →
+theorem BlockPtr.firstOp!_insertOp {block : BlockPtr} :
+    Rewriter.insertOp ctx newOp ip h₁ h₂ h₃ = some newCtx →
     (block.get! newCtx).firstOp =
     if ip.block! ctx = block ∧ ip.prev! ctx = none then
       some newOp
     else
       (block.get! ctx).firstOp := by
-  simp only [Rewriter.insertOp?]
+  simp only [Rewriter.insertOp]
   grind [cases InsertPoint]
 
-grind_pattern BlockPtr.firstOp!_insertOp? =>
-  Rewriter.insertOp? ctx newOp ip h₁ h₂ h₃, some newCtx, (block.get! newCtx).firstOp
+grind_pattern BlockPtr.firstOp!_insertOp =>
+  Rewriter.insertOp ctx newOp ip h₁ h₂ h₃, some newCtx, (block.get! newCtx).firstOp
 
-theorem BlockPtr.lastOp!_insertOp? {block : BlockPtr} :
-    Rewriter.insertOp? ctx newOp ip h₁ h₂ h₃ = some newCtx →
+theorem BlockPtr.lastOp!_insertOp {block : BlockPtr} :
+    Rewriter.insertOp ctx newOp ip h₁ h₂ h₃ = some newCtx →
     (block.get! newCtx).lastOp =
     if ip.block! ctx = block ∧ ip.next = none then
       some newOp
     else
       (block.get! ctx).lastOp := by
-  simp only [Rewriter.insertOp?]
+  simp only [Rewriter.insertOp]
   grind
 
-grind_pattern BlockPtr.lastOp!_insertOp? =>
-  Rewriter.insertOp? ctx newOp ip h₁ h₂ h₃, some newCtx, (block.get! newCtx).lastOp
+grind_pattern BlockPtr.lastOp!_insertOp =>
+  Rewriter.insertOp ctx newOp ip h₁ h₂ h₃, some newCtx, (block.get! newCtx).lastOp
 
-theorem OperationPtr.prev!_insertOp? {operation : OperationPtr} :
-    Rewriter.insertOp? ctx newOp ip h₁ h₂ h₃ = some newCtx →
+theorem OperationPtr.prev!_insertOp {operation : OperationPtr} :
+    Rewriter.insertOp ctx newOp ip h₁ h₂ h₃ = some newCtx →
     (operation.get! newCtx).prev =
     if operation = ip.next then
       some newOp
@@ -135,14 +135,14 @@ theorem OperationPtr.prev!_insertOp? {operation : OperationPtr} :
       ip.prev! ctx
     else
       (operation.get! ctx).prev := by
-  simp only [Rewriter.insertOp?]
+  simp only [Rewriter.insertOp]
   grind [cases InsertPoint]
 
-grind_pattern OperationPtr.prev!_insertOp? =>
-  Rewriter.insertOp? ctx newOp ip h₁ h₂ h₃, some newCtx, (operation.get! newCtx).prev
+grind_pattern OperationPtr.prev!_insertOp =>
+  Rewriter.insertOp ctx newOp ip h₁ h₂ h₃, some newCtx, (operation.get! newCtx).prev
 
-theorem OperationPtr.next!_insertOp? {operation : OperationPtr} :
-    Rewriter.insertOp? ctx newOp ip h₁ h₂ h₃ = some newCtx →
+theorem OperationPtr.next!_insertOp {operation : OperationPtr} :
+    Rewriter.insertOp ctx newOp ip h₁ h₂ h₃ = some newCtx →
     (operation.get! newCtx).next =
     if operation = ip.prev! ctx then
       some newOp
@@ -150,230 +150,230 @@ theorem OperationPtr.next!_insertOp? {operation : OperationPtr} :
       ip.next
     else
       (operation.get! ctx).next := by
-  simp only [Rewriter.insertOp?]
+  simp only [Rewriter.insertOp]
   grind [cases InsertPoint]
 
-grind_pattern OperationPtr.next!_insertOp? =>
-  Rewriter.insertOp? ctx newOp ip h₁ h₂ h₃, some newCtx, (operation.get! newCtx).next
+grind_pattern OperationPtr.next!_insertOp =>
+  Rewriter.insertOp ctx newOp ip h₁ h₂ h₃, some newCtx, (operation.get! newCtx).next
 
-theorem OperationPtr.parent!_insertOp? {operation : OperationPtr} :
-    Rewriter.insertOp? ctx newOp ip h₁ h₂ h₃ = some newCtx →
+theorem OperationPtr.parent!_insertOp {operation : OperationPtr} :
+    Rewriter.insertOp ctx newOp ip h₁ h₂ h₃ = some newCtx →
     (operation.get! newCtx).parent =
     if operation = newOp then
       ip.block! ctx
     else
       (operation.get! ctx).parent := by
-  simp only [Rewriter.insertOp?]
+  simp only [Rewriter.insertOp]
   grind (gen := 10)
 
-grind_pattern OperationPtr.parent!_insertOp? =>
-  Rewriter.insertOp? ctx newOp ip h₁ h₂ h₃, some newCtx, (operation.get! newCtx).parent
+grind_pattern OperationPtr.parent!_insertOp =>
+  Rewriter.insertOp ctx newOp ip h₁ h₂ h₃, some newCtx, (operation.get! newCtx).parent
 
 @[simp]
-theorem OperationPtr.getOpType!_insertOp? {operation : OperationPtr} :
-    Rewriter.insertOp? ctx newOp ip h₁ h₂ h₃ = some newCtx →
+theorem OperationPtr.getOpType!_insertOp {operation : OperationPtr} :
+    Rewriter.insertOp ctx newOp ip h₁ h₂ h₃ = some newCtx →
     operation.getOpType! newCtx = operation.getOpType! ctx := by
-  simp only [Rewriter.insertOp?]
+  simp only [Rewriter.insertOp]
   grind
 
-grind_pattern OperationPtr.getOpType!_insertOp? =>
-  Rewriter.insertOp? ctx newOp ip h₁ h₂ h₃, some newCtx, operation.getOpType! newCtx
+grind_pattern OperationPtr.getOpType!_insertOp =>
+  Rewriter.insertOp ctx newOp ip h₁ h₂ h₃, some newCtx, operation.getOpType! newCtx
 
 @[simp]
-theorem OperationPtr.attrs!_insertOp? {operation : OperationPtr} :
-    Rewriter.insertOp? ctx newOp ip h₁ h₂ h₃ = some newCtx →
+theorem OperationPtr.attrs!_insertOp {operation : OperationPtr} :
+    Rewriter.insertOp ctx newOp ip h₁ h₂ h₃ = some newCtx →
     (operation.get! newCtx).attrs = (operation.get! ctx).attrs := by
   grind
 
-grind_pattern OperationPtr.attrs!_insertOp? =>
-  Rewriter.insertOp? ctx newOp ip h₁ h₂ h₃, some newCtx, (operation.get! newCtx).attrs
+grind_pattern OperationPtr.attrs!_insertOp =>
+  Rewriter.insertOp ctx newOp ip h₁ h₂ h₃, some newCtx, (operation.get! newCtx).attrs
 
 @[simp]
-theorem OperationPtr.getProperties!_insertOp? {operation : OperationPtr} :
-    Rewriter.insertOp? ctx newOp ip h₁ h₂ h₃ = some newCtx →
+theorem OperationPtr.getProperties!_insertOp {operation : OperationPtr} :
+    Rewriter.insertOp ctx newOp ip h₁ h₂ h₃ = some newCtx →
     operation.getProperties! newCtx opCode = operation.getProperties! ctx opCode := by
-  simp only [Rewriter.insertOp?]
+  simp only [Rewriter.insertOp]
   grind
 
-grind_pattern OperationPtr.getProperties!_insertOp? =>
-  Rewriter.insertOp? ctx newOp ip h₁ h₂ h₃, some newCtx, operation.getProperties! newCtx opCode
+grind_pattern OperationPtr.getProperties!_insertOp =>
+  Rewriter.insertOp ctx newOp ip h₁ h₂ h₃, some newCtx, operation.getProperties! newCtx opCode
 
 @[simp]
-theorem OperationPtr.getNumResults!_insertOp? {operation : OperationPtr} :
-    Rewriter.insertOp? ctx newOp ip h₁ h₂ h₃ = some newCtx →
+theorem OperationPtr.getNumResults!_insertOp {operation : OperationPtr} :
+    Rewriter.insertOp ctx newOp ip h₁ h₂ h₃ = some newCtx →
     operation.getNumResults! newCtx = operation.getNumResults! ctx := by
-  simp only [Rewriter.insertOp?]
+  simp only [Rewriter.insertOp]
   grind
 
-grind_pattern OperationPtr.getNumResults!_insertOp? =>
-  Rewriter.insertOp? ctx newOp ip h₁ h₂ h₃, some newCtx, operation.getNumResults! newCtx
+grind_pattern OperationPtr.getNumResults!_insertOp =>
+  Rewriter.insertOp ctx newOp ip h₁ h₂ h₃, some newCtx, operation.getNumResults! newCtx
 
 @[simp]
-theorem OpResultPtr.get!_insertOp? {opResult : OpResultPtr} :
-    Rewriter.insertOp? ctx newOp ip h₁ h₂ h₃ = some newCtx →
+theorem OpResultPtr.get!_insertOp {opResult : OpResultPtr} :
+    Rewriter.insertOp ctx newOp ip h₁ h₂ h₃ = some newCtx →
     opResult.get! newCtx = opResult.get! ctx := by
-  simp only [Rewriter.insertOp?]
+  simp only [Rewriter.insertOp]
   grind
 
-grind_pattern OpResultPtr.get!_insertOp? =>
-  Rewriter.insertOp? ctx newOp ip h₁ h₂ h₃, some newCtx, opResult.get! newCtx
+grind_pattern OpResultPtr.get!_insertOp =>
+  Rewriter.insertOp ctx newOp ip h₁ h₂ h₃, some newCtx, opResult.get! newCtx
 
 @[simp]
-theorem OperationPtr.getNumOperands!_insertOp? {operation : OperationPtr} :
-    Rewriter.insertOp? ctx newOp ip h₁ h₂ h₃ = some newCtx →
+theorem OperationPtr.getNumOperands!_insertOp {operation : OperationPtr} :
+    Rewriter.insertOp ctx newOp ip h₁ h₂ h₃ = some newCtx →
     operation.getNumOperands! newCtx = operation.getNumOperands! ctx := by
-  simp only [Rewriter.insertOp?]
+  simp only [Rewriter.insertOp]
   grind
 
-grind_pattern OperationPtr.getNumOperands!_insertOp? =>
-  Rewriter.insertOp? ctx newOp ip h₁ h₂ h₃, some newCtx, operation.getNumOperands! newCtx
+grind_pattern OperationPtr.getNumOperands!_insertOp =>
+  Rewriter.insertOp ctx newOp ip h₁ h₂ h₃, some newCtx, operation.getNumOperands! newCtx
 
 @[simp]
-theorem OpOperandPtr.get!_insertOp? {operand : OpOperandPtr} :
-    Rewriter.insertOp? ctx newOp ip h₁ h₂ h₃ = some newCtx →
+theorem OpOperandPtr.get!_insertOp {operand : OpOperandPtr} :
+    Rewriter.insertOp ctx newOp ip h₁ h₂ h₃ = some newCtx →
     operand.get! newCtx = operand.get! ctx := by
-  simp only [Rewriter.insertOp?]
+  simp only [Rewriter.insertOp]
   grind
 
-grind_pattern OpOperandPtr.get!_insertOp? =>
-  Rewriter.insertOp? ctx newOp ip h₁ h₂ h₃, some newCtx, operand.get! newCtx
+grind_pattern OpOperandPtr.get!_insertOp =>
+  Rewriter.insertOp ctx newOp ip h₁ h₂ h₃, some newCtx, operand.get! newCtx
 
 @[simp]
-theorem OperationPtr.getOperands!_insertOp? {operation : OperationPtr} :
-    Rewriter.insertOp? ctx newOp ip h₁ h₂ h₃ = some newCtx →
+theorem OperationPtr.getOperands!_insertOp {operation : OperationPtr} :
+    Rewriter.insertOp ctx newOp ip h₁ h₂ h₃ = some newCtx →
     operation.getOperands! newCtx = operation.getOperands! ctx := by
-  simp only [Rewriter.insertOp?]
+  simp only [Rewriter.insertOp]
   grind
 
-grind_pattern OperationPtr.getOperands!_insertOp? =>
-  Rewriter.insertOp? ctx newOp ip h₁ h₂ h₃, some newCtx, operation.getOperands! newCtx
+grind_pattern OperationPtr.getOperands!_insertOp =>
+  Rewriter.insertOp ctx newOp ip h₁ h₂ h₃, some newCtx, operation.getOperands! newCtx
 
 @[simp]
-theorem OperationPtr.getNumSuccessors!_insertOp? {operation : OperationPtr} :
-    Rewriter.insertOp? ctx newOp ip h₁ h₂ h₃ = some newCtx →
+theorem OperationPtr.getNumSuccessors!_insertOp {operation : OperationPtr} :
+    Rewriter.insertOp ctx newOp ip h₁ h₂ h₃ = some newCtx →
     operation.getNumSuccessors! newCtx = operation.getNumSuccessors! ctx := by
-  simp only [Rewriter.insertOp?]
+  simp only [Rewriter.insertOp]
   grind
 
-grind_pattern OperationPtr.getNumSuccessors!_insertOp? =>
-  Rewriter.insertOp? ctx newOp ip h₁ h₂ h₃, some newCtx, operation.getNumSuccessors! newCtx
+grind_pattern OperationPtr.getNumSuccessors!_insertOp =>
+  Rewriter.insertOp ctx newOp ip h₁ h₂ h₃, some newCtx, operation.getNumSuccessors! newCtx
 
 @[simp]
-theorem BlockOperandPtr.get!_insertOp? {operand : BlockOperandPtr} :
-    Rewriter.insertOp? ctx newOp ip h₁ h₂ h₃ = some newCtx →
+theorem BlockOperandPtr.get!_insertOp {operand : BlockOperandPtr} :
+    Rewriter.insertOp ctx newOp ip h₁ h₂ h₃ = some newCtx →
     operand.get! newCtx = operand.get! ctx := by
-  simp only [Rewriter.insertOp?]
+  simp only [Rewriter.insertOp]
   grind
 
-grind_pattern BlockOperandPtr.get!_insertOp? =>
-  Rewriter.insertOp? ctx newOp ip h₁ h₂ h₃, some newCtx, operand.get! newCtx
+grind_pattern BlockOperandPtr.get!_insertOp =>
+  Rewriter.insertOp ctx newOp ip h₁ h₂ h₃, some newCtx, operand.get! newCtx
 
 @[simp]
-theorem OperationPtr.getSuccessor!_insertOp? {operation : OperationPtr} :
-    Rewriter.insertOp? ctx newOp ip h₁ h₂ h₃ = some newCtx →
+theorem OperationPtr.getSuccessor!_insertOp {operation : OperationPtr} :
+    Rewriter.insertOp ctx newOp ip h₁ h₂ h₃ = some newCtx →
     operation.getSuccessor! newCtx index = operation.getSuccessor! ctx index := by
   grind [OperationPtr.getSuccessor!_def]
 
-grind_pattern OperationPtr.getSuccessor!_insertOp? =>
-  Rewriter.insertOp? ctx newOp ip h₁ h₂ h₃, some newCtx, operation.getSuccessor! newCtx index
+grind_pattern OperationPtr.getSuccessor!_insertOp =>
+  Rewriter.insertOp ctx newOp ip h₁ h₂ h₃, some newCtx, operation.getSuccessor! newCtx index
 
 @[simp]
-theorem OperationPtr.getSuccessors!_insertOp? {operation : OperationPtr} :
-    Rewriter.insertOp? ctx newOp ip h₁ h₂ h₃ = some newCtx →
+theorem OperationPtr.getSuccessors!_insertOp {operation : OperationPtr} :
+    Rewriter.insertOp ctx newOp ip h₁ h₂ h₃ = some newCtx →
     operation.getSuccessors! newCtx = operation.getSuccessors! ctx := by
   grind [OperationPtr.getSuccessors!_def]
 
-grind_pattern OperationPtr.getSuccessors!_insertOp? =>
-  Rewriter.insertOp? ctx newOp ip h₁ h₂ h₃, some newCtx, operation.getSuccessors! newCtx
+grind_pattern OperationPtr.getSuccessors!_insertOp =>
+  Rewriter.insertOp ctx newOp ip h₁ h₂ h₃, some newCtx, operation.getSuccessors! newCtx
 
 @[simp]
-theorem OperationPtr.getNumRegions!_insertOp? {operation : OperationPtr} :
-    Rewriter.insertOp? ctx newOp ip h₁ h₂ h₃ = some newCtx →
+theorem OperationPtr.getNumRegions!_insertOp {operation : OperationPtr} :
+    Rewriter.insertOp ctx newOp ip h₁ h₂ h₃ = some newCtx →
     operation.getNumRegions! newCtx = operation.getNumRegions! ctx := by
-  simp only [Rewriter.insertOp?]
+  simp only [Rewriter.insertOp]
   grind
 
-grind_pattern OperationPtr.getNumRegions!_insertOp? =>
-  Rewriter.insertOp? ctx newOp ip h₁ h₂ h₃, some newCtx, operation.getNumRegions! newCtx
+grind_pattern OperationPtr.getNumRegions!_insertOp =>
+  Rewriter.insertOp ctx newOp ip h₁ h₂ h₃, some newCtx, operation.getNumRegions! newCtx
 
 @[simp]
-theorem OperationPtr.getRegion!_insertOp? {operation : OperationPtr} :
-    Rewriter.insertOp? ctx newOp ip h₁ h₂ h₃ = some newCtx →
+theorem OperationPtr.getRegion!_insertOp {operation : OperationPtr} :
+    Rewriter.insertOp ctx newOp ip h₁ h₂ h₃ = some newCtx →
     operation.getRegion! newCtx idx = operation.getRegion! ctx idx := by
-  simp only [Rewriter.insertOp?]
+  simp only [Rewriter.insertOp]
   grind
 
-grind_pattern OperationPtr.getRegion!_insertOp? =>
-  Rewriter.insertOp? ctx newOp ip h₁ h₂ h₃, some newCtx, operation.getRegion! newCtx idx
+grind_pattern OperationPtr.getRegion!_insertOp =>
+  Rewriter.insertOp ctx newOp ip h₁ h₂ h₃, some newCtx, operation.getRegion! newCtx idx
 
 @[simp]
-theorem BlockOperandPtrPtr.get!_insertOp? {operandPtr : BlockOperandPtrPtr} :
-    Rewriter.insertOp? ctx newOp ip h₁ h₂ h₃ = some newCtx →
+theorem BlockOperandPtrPtr.get!_insertOp {operandPtr : BlockOperandPtrPtr} :
+    Rewriter.insertOp ctx newOp ip h₁ h₂ h₃ = some newCtx →
     operandPtr.get! newCtx = operandPtr.get! ctx := by
-  simp only [Rewriter.insertOp?]
+  simp only [Rewriter.insertOp]
   grind
 
-grind_pattern BlockOperandPtrPtr.get!_insertOp? =>
-  Rewriter.insertOp? ctx newOp ip h₁ h₂ h₃, some newCtx, operandPtr.get! newCtx
+grind_pattern BlockOperandPtrPtr.get!_insertOp =>
+  Rewriter.insertOp ctx newOp ip h₁ h₂ h₃, some newCtx, operandPtr.get! newCtx
 
 @[simp]
-theorem BlockPtr.getNumArguments!_insertOp? {block : BlockPtr} :
-    Rewriter.insertOp? ctx newOp ip h₁ h₂ h₃ = some newCtx →
+theorem BlockPtr.getNumArguments!_insertOp {block : BlockPtr} :
+    Rewriter.insertOp ctx newOp ip h₁ h₂ h₃ = some newCtx →
     block.getNumArguments! newCtx = block.getNumArguments! ctx := by
-  simp only [Rewriter.insertOp?]
+  simp only [Rewriter.insertOp]
   grind
 
-grind_pattern BlockPtr.getNumArguments!_insertOp? =>
-  Rewriter.insertOp? ctx newOp ip h₁ h₂ h₃, some newCtx, block.getNumArguments! newCtx
+grind_pattern BlockPtr.getNumArguments!_insertOp =>
+  Rewriter.insertOp ctx newOp ip h₁ h₂ h₃, some newCtx, block.getNumArguments! newCtx
 
 @[simp]
-theorem BlockArgumentPtr.get!_insertOp? {blockArg : BlockArgumentPtr} :
-    Rewriter.insertOp? ctx newOp ip h₁ h₂ h₃ = some newCtx →
+theorem BlockArgumentPtr.get!_insertOp {blockArg : BlockArgumentPtr} :
+    Rewriter.insertOp ctx newOp ip h₁ h₂ h₃ = some newCtx →
     blockArg.get! newCtx = blockArg.get! ctx := by
-  simp only [Rewriter.insertOp?]
+  simp only [Rewriter.insertOp]
   grind
 
-grind_pattern BlockArgumentPtr.get!_insertOp? =>
-  Rewriter.insertOp? ctx newOp ip h₁ h₂ h₃, some newCtx, blockArg.get! newCtx
+grind_pattern BlockArgumentPtr.get!_insertOp =>
+  Rewriter.insertOp ctx newOp ip h₁ h₂ h₃, some newCtx, blockArg.get! newCtx
 
 @[simp]
-theorem RegionPtr.get!_insertOp? {region : RegionPtr} :
-    Rewriter.insertOp? ctx newOp ip h₁ h₂ h₃ = some newCtx →
+theorem RegionPtr.get!_insertOp {region : RegionPtr} :
+    Rewriter.insertOp ctx newOp ip h₁ h₂ h₃ = some newCtx →
     region.get! newCtx = region.get! ctx := by
-  simp only [Rewriter.insertOp?]
+  simp only [Rewriter.insertOp]
   grind
 
-grind_pattern RegionPtr.get!_insertOp? =>
-  Rewriter.insertOp? ctx newOp ip h₁ h₂ h₃, some newCtx, region.get! newCtx
+grind_pattern RegionPtr.get!_insertOp =>
+  Rewriter.insertOp ctx newOp ip h₁ h₂ h₃, some newCtx, region.get! newCtx
 
 @[simp]
-theorem ValuePtr.getFirstUse!_insertOp? {value : ValuePtr} :
-    Rewriter.insertOp? ctx newOp ip h₁ h₂ h₃ = some newCtx →
+theorem ValuePtr.getFirstUse!_insertOp {value : ValuePtr} :
+    Rewriter.insertOp ctx newOp ip h₁ h₂ h₃ = some newCtx →
     value.getFirstUse! newCtx = value.getFirstUse! ctx := by
-  simp only [Rewriter.insertOp?]
+  simp only [Rewriter.insertOp]
   grind
 
-grind_pattern ValuePtr.getFirstUse!_insertOp? =>
-  Rewriter.insertOp? ctx newOp ip h₁ h₂ h₃, some newCtx, value.getFirstUse! newCtx
+grind_pattern ValuePtr.getFirstUse!_insertOp =>
+  Rewriter.insertOp ctx newOp ip h₁ h₂ h₃, some newCtx, value.getFirstUse! newCtx
 
-theorem ValuePtr.getType!_insertOp? {value : ValuePtr} :
-    Rewriter.insertOp? ctx newOp ip h₁ h₂ h₃ = some newCtx →
+theorem ValuePtr.getType!_insertOp {value : ValuePtr} :
+    Rewriter.insertOp ctx newOp ip h₁ h₂ h₃ = some newCtx →
     value.getType! newCtx = value.getType! ctx := by
   grind
 
-grind_pattern ValuePtr.getType!_insertOp? =>
-  Rewriter.insertOp? ctx newOp ip h₁ h₂ h₃, some newCtx, value.getType! newCtx
+grind_pattern ValuePtr.getType!_insertOp =>
+  Rewriter.insertOp ctx newOp ip h₁ h₂ h₃, some newCtx, value.getType! newCtx
 
 @[simp]
-theorem OpOperandPtrPtr.get!_insertOp? {opOperandPtr : OpOperandPtrPtr} :
-    Rewriter.insertOp? ctx newOp ip h₁ h₂ h₃ = some newCtx →
+theorem OpOperandPtrPtr.get!_insertOp {opOperandPtr : OpOperandPtrPtr} :
+    Rewriter.insertOp ctx newOp ip h₁ h₂ h₃ = some newCtx →
     opOperandPtr.get! newCtx = opOperandPtr.get! ctx := by
-  simp only [Rewriter.insertOp?]
+  simp only [Rewriter.insertOp]
   grind
 
-grind_pattern OpOperandPtrPtr.get!_insertOp? =>
-  Rewriter.insertOp? ctx newOp ip h₁ h₂ h₃, some newCtx, opOperandPtr.get! newCtx
+grind_pattern OpOperandPtrPtr.get!_insertOp =>
+  Rewriter.insertOp ctx newOp ip h₁ h₂ h₃, some newCtx, opOperandPtr.get! newCtx
 
-end Rewriter.insertOp?
+end Rewriter.insertOp
 
 end Veir
